theories/rust_typing/integration_tests.v
@@ -182,8 +182,8 @@ Section test.
   Next Obligation. ex_t_solve_timeless. Qed.
   Local Definition Pty := (∃; Pdef, int I32)%I.
 
-  Local Definition P_b := λ (π : thread_id) (x : Z) (y : Z), (∃ (z : Z) (l : loc), ⌜x = (y + z)%Z⌝ ∗ ⌜(0 < x)%Z⌝ ∗ l ◁ₗ[π, Owned true] #42%Z @ (◁ int I32))%I : iProp Σ.
-  Local Definition S_b := λ (π : thread_id) (κ : lft) (x : Z) (y : Z), (∃ (z : Z) (l : loc), ⌜x = (y + z)%Z⌝ ∗ ⌜(0 < x)%Z⌝ ∗ guarded (l ◁ₗ[π, Shared κ] #42%Z @ (◁ int I32)))%I : iProp Σ.
+  Local Definition P_b := λ (π : thread_id) (x : Z) (y : Z), (∃ (z : Z) (l : loc), ⌜x = (y + z)%Z⌝ ∗ ⌜(0 < x)%Z⌝ ∗ guarded true (l ◁ₗ[π, Owned false] #42%Z @ (◁ int I32)))%I : iProp Σ.
+  Local Definition S_b := λ (π : thread_id) (κ : lft) (x : Z) (y : Z), (∃ (z : Z) (l : loc), ⌜x = (y + z)%Z⌝ ∗ ⌜(0 < x)%Z⌝ ∗ guarded false (l ◁ₗ[π, Shared κ] #42%Z @ (◁ int I32)))%I : iProp Σ.
 
   Local Program Definition Adef := mk_ex_inv_def P_b S_b [] [] _ _ _.
   Next Obligation. ex_t_solve_persistent. Qed.
