theories/rust_typing/manual.v
@@ -1,5 +1,5 @@
 From iris.proofmode Require Import coq_tactics reduction string_ident.
-From refinedrust Require Import programs array.array automation value.
+From refinedrust Require Import programs program_rules array.array automation value.
 From refinedrust Require Import options.
 
 
@@ -363,53 +363,38 @@ Section updateable_rules.
     iFrame. iApply ("Hs" with "Hnamed").
   Qed.
 
-  (** Strip a later from a type assignment *)
-  Lemma updateable_ltype_strip_later l  :
+  (** Add a guard to a type assignment *)
+  Lemma updateable_ltype_add_guard l prepaid :
     (find_in_context (FindLoc l) (λ '(existT rt (lt, r, bk, π)),
-      ⌜bk = Owned true⌝ ∗ ⌜match ltype_lty _ lt with
-       | OpenedLty _ _ _ _ _ | CoreableLty _ _ | ShadowedLty _ _ _ | OpenedNaLty _ _ _ _ => False
-       | _ => True
-       end⌝ ∗
-      (l ◁ₗ[π, Owned false] r @ lt -∗ updateable_core updateable_E updateable_L)))
+      prove_with_subtype updateable_E updateable_L false ProveDirect (maybe_creds prepaid) (λ L2 _ R,
+      R -∗ guarded prepaid (l ◁ₗ[π, bk] r @ lt) -∗ updateable_core updateable_E L2)))
     ⊢ P.
   Proof.
     unfold find_in_context,FindLoc. simpl.
     iIntros "(%x & Ha)".
     destruct x as [rt (((lt & r) & bk) & π)].
-    iDestruct "Ha" as "(Hl & -> & % & HT)".
-    unshelve iApply add_updateable; first apply _.
-    iIntros "CTX HE HL".
-    iPoseProof (ltype_own_Owned_true_false with "Hl") as "(Hcred & Hl)"; first done.
-    iDestruct "Hcred" as "((Hcred1 & Hcred) & _)".
-    iApply (lc_fupd_add_later with "Hcred1").
-    iNext. iModIntro. iExists updateable_L. iFrame.
-    by iApply "HT".
-  Qed.
-
-  (** Add a later to a type assignment *)
-  Lemma updateable_ltype_add_later l  :
-    (find_in_context (FindLoc l) (λ '(existT rt (lt, r, bk, π)),
-      ⌜bk = Owned false⌝ ∗
-      ⌜match ltype_lty _ lt with
-       | OpenedLty _ _ _ _ _ | CoreableLty _ _ | ShadowedLty _ _ _ | OpenedNaLty _ _ _ _ => False
-       | _ => True
-       end⌝ ∗
-      prove_with_subtype updateable_E updateable_L false ProveDirect (have_creds) (λ L2 _ R,
-      R -∗ l ◁ₗ[π, Owned true] r @ lt -∗ updateable_core updateable_E L2)))
-    ⊢ P.
-  Proof.
-    unfold find_in_context,FindLoc. simpl.
-    iIntros "(%x & Ha)".
-    destruct x as [rt (((lt & r) & bk) & π)].
-    iDestruct "Ha" as "(Hl & -> & % & HT)".
+    iDestruct "Ha" as "(Hl & HT)".
     unshelve iApply add_updateable; first apply _.
     iIntros "#CTX HE HL".
     unfold prove_with_subtype.
     iMod ("HT" with "[] [] [] CTX HE HL") as "(%L2 & % & %R & Ha & HL & HT)"; [done.. | ].
     simpl. iMod "Ha" as "(Hcred & HR)".
-    iPoseProof (ltype_own_Owned_false_true with "Hl Hcred") as "Hl"; first done.
     iFrame.
-    iApply ("HT" with "HR Hl").
+    iApply ("HT" with "HR [Hcred Hl]").
+    rewrite /guarded.
+    iFrame.
+  Qed.
+
+  Lemma updateable_strip_guards :
+    iterate_with_hooks updateable_E updateable_L strip_guarded (λ L,
+      updateable_core updateable_E L)
+    ⊢ P.
+  Proof.
+    iIntros "HT". unshelve iApply add_updateable; first apply _.
+    iIntros "#CTX HE HL".
+    unfold iterate_with_hooks.
+    iMod ("HT" with "[] HE HL") as "Ha"; first done.
+    done.
   Qed.
 
   (** Discard the opened invariant on an owned location, removing the obligation to re-establish the invariant *)
